Wavelet/Compile.lean
@@ -1,0 +1,137 @@
+import Wavelet.Op
+import Wavelet.Seq
+import Wavelet.Dataflow
+
+/-! A compiler from Seq to dataflow. -/
+
+namespace Wavelet.Compile
+
+open Op Seq Dataflow
+
+universe u
+variable (Op : Type u) (χ : Type u) (V S)
+variable [Arity Op] [DecidableEq χ] [instInterp : Interp Op V S]
+
+/--
+Compiles an expression to a list of atomic processes, with
+exactly `m + n + 1` outputs, where `m` is the number of parameters
+of the encompassing function, `n` is the number of return values,
+and the extra output is a Boolean indicating whether the expression
+chooses to perform a tail call (with `m` arguments) or return
+`n` final values.
+-/
+def compileExpr
+  (wf : m > 0 ∧ n > 0) -- Additional well-formedness condition
+  (definedVars : List χ)
+  (pathConds : List (Bool × ChanName χ))
+  : Expr Op χ m n → AtomicProcs Op (ChanName χ) V
+  | .ret vars =>
+    let chans := vars.map liveVar
+    let act := chans[0] -- Use the first return value as an activation signal
+    [
+      .forward chans retChans,
+      -- No tail recursion, so we send junk values for the tail arguments
+      -- and send `false` on the tail condition channel.
+      .const (Interp.junkVal Op S) act tailArgs,
+      .const (Interp.falseVal Op S) act #v[.tail_cond pathConds]
+    ]
+  | .tail vars =>
+    let chans := vars.map liveVar
+    let act := chans[0]
+    [
+      .const (Interp.junkVal Op S) act retChans,
+      .forward chans tailArgs,
+      .const (Interp.trueVal Op S) act #v[.tail_cond pathConds]
+    ]
+  | .op o args rets cont =>
+    let inputChans := args.map liveVar
+    let (definedVars', outputChans) := newVars rets
+    (.op o inputChans outputChans) :: compileExpr wf definedVars' pathConds cont
+  | .br cond left right =>
+    let condChan := liveVar cond
+    let leftConds := (true, condChan.1) :: pathConds
+    let rightConds := (false, condChan.1) :: pathConds
+    let leftComp := compileExpr wf definedVars leftConds left
+    let rightComp := compileExpr wf definedVars rightConds right
+    let allVars := definedVars.eraseDups.toArray.toVector
+    [
+      -- Steer all live variables
+      .steer true condChan
+        (allVars.map λ v => empty (.var v (definedVars.count v) pathConds))
+        (allVars.map λ v => .var v (definedVars.count v) leftConds),
+      .steer false condChan
+        (allVars.map λ v => empty (.var v (definedVars.count v) pathConds))
+        (allVars.map λ v => .var v (definedVars.count v) rightConds),
+      -- Forward the condition again to the merge
+      -- (extra forward for a simpler simulation relation)
+      .forward #v[condChan] #v[.merge_cond condChan.1],
+    ] ++ leftComp ++ rightComp ++ [
+      -- Merge tail call conditions, return values and tail call arguments
+      -- from both branches. This is done at the end so that we can keep
+      -- the graph as "acyclic" as possible.
+      brMerge m n condChan.1 [] pathConds
+    ]
+  where
+    empty := ChanBuf.empty _
+    liveVar v := empty (.var v (definedVars.count v) pathConds)
+    retChans := (Vector.range n).map λ i => .dest i pathConds
+    tailArgs := (Vector.range m).map λ i => .tail_arg i pathConds
+    newVars {k} (vs : Vector χ k) : List χ × Vector (ChanName χ) k :=
+      (
+        definedVars ++ vs.toList,
+        vs.map λ v => .var v (definedVars.count v + 1) pathConds
+      )
+    brMerge m n condName condBuf pathConds :=
+      let leftConds := (true, condName) :: pathConds
+      let rightConds := (false, condName) :: pathConds
+      let leftResults := #v[empty (.tail_cond leftConds)] ++
+        ((Vector.range n).map λ i => empty (.dest i leftConds)) ++
+        ((Vector.range m).map λ i => empty (.tail_arg i leftConds))
+      let rightResults := #v[empty (.tail_cond rightConds)] ++
+        ((Vector.range n).map λ i => empty (.dest i rightConds)) ++
+        ((Vector.range m).map λ i => empty (.tail_arg i rightConds))
+      let results := #v[ChanName.tail_cond pathConds] ++
+        ((Vector.range n).map λ i => ChanName.dest i pathConds) ++
+        ((Vector.range m).map λ i => ChanName.tail_arg i pathConds)
+      .merge (.merge_cond condName, condBuf)
+        leftResults
+        rightResults
+        results
+
+/--
+Compiles a function to a process with `m` inputs and `n` outputs.
+
+Most of the compiled process should be a DAG, except for the back
+edges of channels with the name `.tail_cond []` or `.tail_arg i []`.
+-/
+def compileFn
+  (fn : Fn Op χ m n) : Proc Op (ChanName χ) V m n
+  :=
+  {
+    inputs := fn.params.map λ v => .var v 0 [],
+    outputs := (Vector.range n).map λ i => .empty _ (.final_tail_arg i),
+    atoms := initCarry :: (bodyComp ++ resultSteers m n)
+  }
+  where
+    -- A carry gate to merge initial values and tail call arguments
+    initCarry :=
+      .carry false
+        (.empty _ (.tail_cond []))
+        (fn.params.map λ v => .empty _ (.var v 0 []))
+        ((Vector.range m).map λ i => .empty _ (.final_tail_arg i))
+        (fn.params.map λ v => .var v 1 [])
+    bodyComp := compileExpr Op χ V S fn.NonEmptyIO fn.params.toList [] fn.body
+    resultSteers m n := [
+      -- If tail condition is true, discard the junk return values
+      .steer false
+        (.empty _ (.tail_cond []))
+        ((Vector.range n).map λ i => .empty _ (.dest i []))
+        ((Vector.range n).map λ i => .final_dest i),
+      -- If tail condition is false, discard the junk tail arguments
+      .steer true
+        (.empty _ (.tail_cond []))
+        ((Vector.range m).map λ i => .empty _ (.tail_arg i []))
+        ((Vector.range m).map λ i => .final_tail_arg i),
+    ]
+
+end Wavelet.Compile
