Wavelet/Dataflow.lean
@@ -1,0 +1,150 @@
+import Mathlib.Logic.Relation
+import Wavelet.Op
+
+/-! Syntax and semantics for a simple dataflow calculus. -/
+
+namespace Wavelet.Dataflow
+
+open Op
+
+universe u
+variable (Op : Type u) (χ : Type u)
+variable [Arity Op]
+variable [DecidableEq χ]
+
+/- A channel name attached with a value buffer. -/
+abbrev ChanBuf V := χ × List V
+
+def ChanBuf.empty (v : χ) : ChanBuf χ V := (v, [])
+
+def ChanBuf.push (updates : List (χ × V)) (buf : ChanBuf χ V) : ChanBuf χ V :=
+  updates.foldl (λ buf (var, val) =>
+    if buf.1 = var then (buf.1, buf.2.concat val)
+    else (buf.1, buf.2)) buf
+
+def ChanBuf.pushAll (updates : List (χ × V))
+  (bufs : Vector (ChanBuf χ V) n) : Vector (ChanBuf χ V) n :=
+  bufs.map (ChanBuf.push _ updates)
+
+def ChanBuf.pop (buf : ChanBuf χ V) : Option (V × ChanBuf χ V) :=
+  match buf.2 with
+  | [] => none
+  | v :: vs => some (v, (buf.1, vs))
+
+def ChanBuf.popAll (bufs : Vector (ChanBuf χ V) n) : Option (Vector V n × Vector (ChanBuf χ V) n) := do
+  let res ← bufs.mapM (ChanBuf.pop _)
+  return (res.map Prod.fst, res.map Prod.snd)
+
+/-- Dataflow operators. -/
+inductive AtomicProc V where
+  | op (op : Op) (inputs : Vector (ChanBuf χ V) (Arity.ι op)) (outputs : Vector χ (Arity.ω op))
+  | steer (flavor : Bool) (decider : ChanBuf χ V) (inputs : Vector (ChanBuf χ V) n) (outputs : Vector χ n)
+  | carry (inLoop : Bool)
+    (decider : ChanBuf χ V)
+    (inputs₁ : Vector (ChanBuf χ V) n) (inputs₂ : Vector (ChanBuf χ V) n)
+    (outputs : Vector χ n)
+  | merge (decider : ChanBuf χ V)
+    (inputs₁ : Vector (ChanBuf χ V) n) (inputs₂ : Vector (ChanBuf χ V) n)
+    (outputs : Vector χ n)
+  | forward (inputs : Vector (ChanBuf χ V) n) (outputs : Vector χ n)
+  | const (c : V) (act : ChanBuf χ V) (outputs : Vector χ n)
+  deriving Repr
+
+def AtomicProc.inputs (ap : AtomicProc Op χ V) : List (ChanBuf χ V) :=
+  match ap with
+  | .op _ inputs _ => inputs.toList
+  | .steer _ decider inputs _ => [decider] ++ inputs.toList
+  | .carry _ decider input₁ input₂ _ => [decider] ++ input₁.toList ++ input₂.toList
+  | .merge decider input₁ input₂ _ => [decider] ++ input₁.toList ++ input₂.toList
+  | .forward inputs _ => inputs.toList
+  | .const _ act _ => [act]
+
+def AtomicProc.outputs (ap : AtomicProc Op χ V) : List χ :=
+  match ap with
+  | .op _ _ outputs => outputs.toList
+  | .steer _ _ _ outputs => outputs.toList
+  | .carry _ _ _ _ outputs => outputs.toList
+  | .merge _ _ _ outputs => outputs.toList
+  | .forward _ outputs => outputs.toList
+  | .const _ _ outputs => outputs.toList
+
+abbrev AtomicProcs V := List (AtomicProc Op χ V)
+
+/-- `Proc _ m n` is a process with `m` inputs and `n` outputs. -/
+structure Proc V (m : Nat) (n : Nat) where
+  inputs : Vector χ m
+  outputs : Vector (ChanBuf χ V) n
+  atoms : AtomicProcs Op χ V
+
+/- From this point onwards, assume a fixed operator semantics. -/
+variable (V S) [instInterp : Interp Op V S]
+
+def AtomicProc.push (updates : List (χ × V)) : AtomicProc Op χ V → AtomicProc Op χ V
+  | .op o inputs outputs => .op o (pushAll inputs) outputs
+  | .steer flavor decider inputs outputs => .steer flavor (pushOne decider) (pushAll inputs) outputs
+  | .carry inLoop decider inputs₁ inputs₂ outputs =>
+    .carry inLoop (pushOne decider) (pushAll inputs₁) (pushAll inputs₂) outputs
+  | .merge decider inputs₁ inputs₂ outputs =>
+    .merge (pushOne decider) (pushAll inputs₁) (pushAll inputs₂) outputs
+  | .forward inputs outputs => .forward (pushAll inputs) outputs
+  | .const c act outputs => .const c (pushOne act) outputs
+  where
+    pushOne (buf : ChanBuf χ V) := ChanBuf.push _ updates buf
+    pushAll {n} (bufs : Vector (ChanBuf χ V) n) := ChanBuf.pushAll _ updates bufs
+
+def AtomicProcs.pushAll
+  (updates : List (χ × V))
+  (aps : AtomicProcs Op χ V) :
+  AtomicProcs Op χ V :=
+  aps.map (AtomicProc.push _ _ _ updates)
+
+def Proc.push (updates : List (χ × V)) (p : Proc Op χ V m n) : Proc Op χ V m n :=
+  { p with
+    outputs := ChanBuf.pushAll _ updates p.outputs,
+    atoms := AtomicProcs.pushAll _ _ _ updates p.atoms }
+
+structure Config m n where
+  proc : Proc Op χ V m n
+  state : S
+
+/-- Initial process configuration. -/
+def Config.init
+  (proc : Proc Op χ V m n)
+  (state : S)
+  (vars : Vector V m) : Config Op χ V S m n
+  := {
+    proc := proc.push _ _ _ (proc.inputs.zip vars).toList,
+    state,
+  }
+
+inductive Config.Step : Config Op χ V S m n → Config Op χ V S m n → Prop where
+  | step_op
+    {state : S}
+    {inputs : Vector (ChanBuf χ V) (Arity.ι o)} {outputs}
+    (hinputs : ChanBuf.popAll _ inputs = some (inputVals, inputs'))
+    (hop : (instInterp.interp o inputVals).run state = some (outputVals, state')) :
+    Step
+      {
+        proc := {
+          inputs := procInputs,
+          outputs := procOutputs,
+          atoms := ctxLeft ++ [AtomicProc.op o inputs outputs] ++ ctxRight
+        },
+        state,
+      }
+      {
+        proc := {
+          inputs := procInputs,
+          outputs := ChanBuf.pushAll _ (outputs.zip outputVals).toList procOutputs,
+          atoms :=
+            .pushAll _ _ _ (outputs.zip outputVals).toList
+            (ctxLeft ++ [AtomicProc.op o inputs' outputs] ++ ctxRight)
+        },
+        state := state',
+      }
+
+def Config.StepPlus {m n} := @Relation.TransGen (Config Op χ V S m n) (Step Op χ V S)
+
+def Config.StepStar {m n} := @Relation.ReflTransGen (Config Op χ V S m n) (Step Op χ V S)
+
+end Wavelet.Dataflow
