Wavelet/Simulation.lean
@@ -1,0 +1,399 @@
+import Mathlib.Data.List.Basic
+import Mathlib.Logic.Relation
+
+import Wavelet.Op
+import Wavelet.Seq
+import Wavelet.Dataflow
+import Wavelet.Compile
+
+open Wavelet.Op
+
+universe u
+variable (Op : Type u) (χ : Type u) (V S)
+variable [Arity Op] [DecidableEq χ] [instInterp : Interp Op V S]
+
+/-! Simulation proofs. -/
+
+/-! Some utilities for the simulation invariants. -/
+namespace Wavelet.Seq
+
+/-- Checks if the channel name is a variable and it has
+a different suffix than the given path condition. -/
+def ChanName.HasDiffPathSuffix (pathConds : List (Bool × ChanName χ)) (name : ChanName χ) : Prop :=
+  match name with
+  | .var _ _ pathConds' => ∀ ext, ext ++ pathConds ≠ pathConds'
+  | _ => True
+
+end Wavelet.Seq
+
+/-! Some utilities for the simulation invariants. -/
+namespace Wavelet.Dataflow
+
+open Wavelet.Seq
+
+def AtomicProc.HasInput (ap : AtomicProc Op χ V) (v : χ) : Prop :=
+  ∃ inp ∈ ap.inputs, inp.1 = v
+
+def AtomicProc.HasInputWithBuf (ap : AtomicProc Op χ V) (v : χ) (buf : List V) : Prop :=
+  ∃ inp ∈ ap.inputs, inp = (v, buf)
+
+def AtomicProc.HasEmptyInputs (ap : AtomicProc Op χ V) : Prop :=
+  ∀ inp ∈ ap.inputs, inp.2 = []
+
+def ChanBuf.MatchModBuffer (buf₁ buf₂ : ChanBuf χ V) : Prop := buf₁.1 = buf₂.1
+
+def AtomicProc.MatchModBuffers : AtomicProc Op χ V → AtomicProc Op χ V → Prop
+  | .op o₁ inputs₁ outputs₁, .op o₂ inputs₂ outputs₂ =>
+    o₁ = o₂ ∧
+    List.Forall₂ MatchBuf inputs₁.toList inputs₂.toList ∧
+    outputs₁.toList = outputs₂.toList
+  | .steer flavor₁ decider₁ inputs₁ outputs₁, .steer flavor₂ decider₂ inputs₂ outputs₂ =>
+    flavor₁ = flavor₂ ∧
+    decider₁.1 = decider₂.1 ∧
+    List.Forall₂ MatchBuf inputs₁.toList inputs₂.toList ∧
+    outputs₁.toList = outputs₂.toList
+  | .carry inLoop₁ decider₁ inputs₁₁ inputs₁₂ outputs₁,
+    .carry inLoop₂ decider₂ inputs₂₁ inputs₂₂ outputs₂ =>
+    inLoop₁ = inLoop₂ ∧
+    decider₁.1 = decider₂.1 ∧
+    List.Forall₂ MatchBuf inputs₁₁.toList inputs₂₁.toList ∧
+    List.Forall₂ MatchBuf inputs₁₂.toList inputs₂₂.toList ∧
+    outputs₁.toList = outputs₂.toList
+  | .merge decider₁ inputs₁₁ inputs₁₂ outputs₁,
+    .merge decider₂ inputs₂₁ inputs₂₂ outputs₂ =>
+    decider₁.1 = decider₂.1 ∧
+    List.Forall₂ MatchBuf inputs₁₁.toList inputs₂₁.toList ∧
+    List.Forall₂ MatchBuf inputs₁₂.toList inputs₂₂.toList ∧
+    outputs₁.toList = outputs₂.toList
+  | .forward inputs₁ outputs₁, .forward inputs₂ outputs₂ =>
+    List.Forall₂ MatchBuf inputs₁.toList inputs₂.toList ∧
+    outputs₁.toList = outputs₂.toList
+  | .const c₁ act₁ outputs₁, .const c₂ act₂ outputs₂ =>
+    c₁ = c₂ ∧ act₁.1 = act₂.1 ∧
+    outputs₁.toList = outputs₂.toList
+  | _, _ => False
+  where
+    @[simp]
+    MatchBuf := ChanBuf.MatchModBuffer _ _
+
+def AtomicProcs.MatchModBuffers (aps₁ aps₂ : AtomicProcs Op χ V) : Prop :=
+  List.Forall₂ (AtomicProc.MatchModBuffers Op χ V) aps₁ aps₂
+
+def AtomicProcs.IsDAG (aps : AtomicProcs Op χ V) : Prop :=
+  ∀ i j, (hi : i < aps.length) → (hj : j ≤ i) →
+    ∀ output ∈ aps[i].outputs, ¬ aps[j].HasInput Op χ V output
+
+def AtomicProcs.HasEmptyInputs (aps : AtomicProcs Op χ V) : Prop :=
+  ∀ ap ∈ aps, ap.HasEmptyInputs Op χ V
+
+def AtomicProc.HasDiffPathSuffix (pathConds : List (Bool × ChanName χ)) (ap : AtomicProc Op (ChanName χ) V) : Prop :=
+  ∀ inp ∈ ap.inputs, inp.1.HasDiffPathSuffix _ pathConds
+
+def AtomicProcs.HasDiffPathSuffix (pathConds : List (Bool × ChanName χ)) (aps : AtomicProcs Op (ChanName χ) V) : Prop :=
+  ∀ ap ∈ aps, ap.HasDiffPathSuffix _ _ _ pathConds
+
+end Wavelet.Dataflow
+
+namespace Wavelet.Simulation
+
+open Op Seq Dataflow Compile
+
+/-- Defines refinement of two transition systems in general. -/
+def Refines
+  {T : Type v} {S : Type w}
+  (c₁ : T) (c₂ : S)
+  (R : T → S → Prop)
+  (Step₁ : T → T → Prop)
+  (Step₂ : S → S → Prop) :=
+  R c₁ c₂ ∧
+  (∀ c₁ c₂ c₁',
+    R c₁ c₂ →
+    Step₁ c₁ c₁' →
+    ∃ c₂', Step₂ c₂ c₂' ∧ R c₁' c₂')
+
+/-- Specific case for a Seq config to refine a dataflow config. -/
+def SeqRefinesDataflow
+  [DecidableEq χ₁] [DecidableEq χ₂]
+  (c₁ : Seq.Config Op χ₁ V S m n)
+  (c₂ : Dataflow.Config Op χ₂ V S m n)
+  (R : Seq.Config Op χ₁ V S m n → Dataflow.Config Op χ₂ V S m n → Prop) : Prop :=
+  Refines c₁ c₂ R (Config.Step Op χ₁ V S) (Config.StepPlus Op χ₂ V S)
+
+/-- The main invariant for proving forward simulation of compilation. -/
+def SimR (ec : Seq.Config Op χ V S m n) (pc : Dataflow.Config Op (ChanName χ) V S m n) : Prop :=
+  ec.estate.state = pc.state ∧
+  -- The process matches the compiled function in shape
+  AtomicProcs.MatchModBuffers _ _ _ pc.proc.atoms (compileFn Op χ V S ec.estate.fn).atoms ∧
+  ∃ (rest : AtomicProcs Op (ChanName χ) V)
+    (carryInLoop : Bool)
+    (carryDecider : ChanBuf (ChanName χ) V)
+    (carryInputs₁ carryInputs₂ : Vector (ChanBuf (ChanName χ) V) m)
+    (carryOutputs : Vector (ChanName χ) m)
+    (ctxLeft ctxCurrent ctxRight : AtomicProcs Op (ChanName χ) V),
+    -- The processes form a DAG if we remove the first carry operator
+    pc.proc.atoms = (.carry carryInLoop carryDecider carryInputs₁ carryInputs₂ carryOutputs) :: rest ∧
+    rest.IsDAG _ _ _ ∧
+    -- States of the first carry gate
+    (¬ carryInLoop → ∀ input ∈ carryInputs₁, ∃ var val, input = (.var var 0 [], [val])) ∧
+    (carryInLoop → ∀ input ∈ carryInputs₁, input.2 = []) ∧
+    -- The processes can be split into three fragments
+    rest = ctxLeft ++ ctxCurrent ++ ctxRight ∧
+    ctxLeft.HasEmptyInputs _ _ _ ∧
+    -- If we have reached the end of execution, nothing else should be executable
+    (∀ vals, ec.expr = .ret vals →
+      ctxCurrent = [] ∧
+      ctxRight = [] ∧
+      -- Same return value in the proc side
+      List.Forall₂ (λ v (_, buf) => buf = [v])
+        vals.toList pc.proc.outputs.toList) ∧
+    -- If we still have a continuation
+    (∀ expr, ec.expr = .cont expr →
+      expr.WellFormed ∧
+      -- The current fragment corresponds to the compilation results
+      AtomicProcs.MatchModBuffers _ _ _
+        ctxCurrent
+        (compileExpr Op χ V S ec.estate.fn.NonEmptyIO ec.estate.definedVars ec.estate.pathConds expr) ∧
+      -- Some constraints about live variables
+      (∀ ap ∈ ctxCurrent, ∀ inp ∈ ap.inputs,
+        -- Check if the channel name corresponds to a live variable
+        -- in the current branch
+        let IsLiveVar (name : ChanName χ) val := ∃ var,
+          ec.estate.vars var = some val ∧
+          name = .var var (ec.estate.definedVars.count var) ec.estate.pathConds
+        -- If it's a live var, the channel buffer should have the corresponding value
+        (∀ val, IsLiveVar inp.1 val → inp.2 = [val]) ∧
+        -- Otherwise it's empty.
+        ((∀ val, ¬ IsLiveVar inp.1 val) → inp.2 = [])) ∧
+      -- The remaining processes in `ctxRight` should be of the form
+      --
+      --   `p₁ ... pₘ || merge || p'₁ ... p'ₖ || merge || ...`
+      --
+      -- i.e., a sequence of processes interspersed with consecutive
+      -- chunks of n merge nodes.
+      -- Furthermore, all processes other than these merges should
+      -- have empty input buffers, and the merges will have exactly
+      -- one Boolean in the decider buffers corresponding to the
+      -- branching decision.
+      (∃ (chunks : List (AtomicProcs Op (ChanName χ) V × AtomicProc Op (ChanName χ) V))
+        (tail : AtomicProcs Op (ChanName χ) V),
+        ctxRight = (joinM (chunks.map (λ (l, r) => l ++ [r]))) ++ tail ∧
+        -- The first half chunks and the tail have empty inputs
+        (∀ chunk₁ chunk₂, (chunk₁, chunk₂) ∈ chunks →
+          chunk₁.HasEmptyInputs _ _ _ ∧
+          chunk₁.HasDiffPathSuffix _ _ _ ec.estate.pathConds) ∧
+        tail.HasEmptyInputs _ _ _ ∧
+        tail.HasDiffPathSuffix _ _ _ ec.estate.pathConds ∧
+        -- The second half chunk corresponds exactly to the merge nodes
+        -- generated along the branches marked in the current `pathConds`.
+        List.Forall₂
+          (λ (_, merge) i =>
+            let (b, cond) := ec.estate.pathConds[i]
+            let prevPathConds := ec.estate.pathConds.drop (i + 1)
+            ∃ v,
+              Interp.asBool Op S v = b ∧
+              -- Same as the original merge gate, except with the corresponding
+              -- branching decision in the decider buffer.
+              merge = compileExpr.brMerge Op _ _ m n cond [v] prevPathConds)
+          chunks
+          (Vector.finRange ec.estate.pathConds.length).toList))
+
+theorem aps_match_mod_bufs_refl
+  {aps : AtomicProcs Op χ V} :
+  AtomicProcs.MatchModBuffers Op χ V aps aps := sorry
+
+theorem aps_push_preserves_shape
+  {aps : AtomicProcs Op χ V} :
+  AtomicProcs.MatchModBuffers Op χ V (AtomicProcs.pushAll Op χ V updates aps) aps := sorry
+
+theorem aps_push_preserves_dag
+  {aps : AtomicProcs Op χ V}
+  (hdag : AtomicProcs.IsDAG Op _ V aps) :
+  AtomicProcs.IsDAG Op _ V (AtomicProcs.pushAll Op χ V updates aps) := sorry
+
+theorem aps_push_commutes_tail
+  {aps : AtomicProcs Op χ V}  :
+  (AtomicProcs.pushAll Op χ V updates aps).tail
+    = AtomicProcs.pushAll Op χ V updates aps.tail := sorry
+
+theorem aps_push_commutes_append
+  {aps₁ aps₂ : AtomicProcs Op χ V} :
+  (AtomicProcs.pushAll Op χ V updates (aps₁ ++ aps₂))
+    = (AtomicProcs.pushAll Op χ V updates aps₁) ++ (AtomicProcs.pushAll Op χ V updates aps₂) := sorry
+
+/-- The result of compilation should be a DAG except for the first carry process. -/
+theorem fn_compile_dag
+  {fn : Fn Op χ m n} :
+  AtomicProcs.IsDAG Op _ V ((compileFn Op χ V S fn).atoms.tail) := sorry
+
+/-- Initial configs satisfy the simulation relation. -/
+theorem sim_init_config
+  (f : Fn Op χ m n)
+  (p : Proc Op (ChanName χ) V m n)
+  (hcomp : compileFn Op χ V S f = p)
+  (s : S)
+  (args : Vector V m) :
+  SimR _ _ _ _
+    (Seq.Config.init _ _ _ _ f s args)
+    (Dataflow.Config.init _ _ _ _ p s args) := by
+  simp only [← hcomp]
+  and_intros
+  · rfl
+  · apply aps_push_preserves_shape
+  · generalize hinitUpdates : ((compileFn Op χ V S f).inputs.zip args).toList = initUpdates
+    exists
+      (Proc.push Op _ _ initUpdates p).atoms.tail,
+      false,
+      (.empty _ (.tail_cond [])),
+      (f.params.map λ v => (ChanBuf.empty _ (.var v 0 [])).push _ initUpdates),
+      ((Vector.range m).map λ i => .empty _ (.final_tail_arg i)),
+      (f.params.map λ v => .var v 1 []),
+      [],
+      AtomicProcs.pushAll Op _ _ initUpdates (compileFn.bodyComp Op χ V S f),
+      AtomicProcs.pushAll Op _ _ initUpdates (compileFn.resultSteers Op χ V m n)
+    and_intros
+    · simp [Dataflow.Config.init, Proc.push, ← hcomp]
+      cases h : (compileFn Op χ V S f).atoms with
+      | nil => simp [compileFn] at h
+      | cons carry rest =>
+        simp [AtomicProcs.pushAll, List.tail, hinitUpdates]
+        -- TODO: Reason about carry substitution
+        simp [compileFn, compileFn.initCarry] at h
+        simp only [← h.1, AtomicProc.push, AtomicProc.push.pushOne]
+        congr 1
+        · sorry
+        · sorry
+        · sorry
+    · simp [Proc.push, ← hcomp]
+      apply aps_push_preserves_dag
+      apply fn_compile_dag
+    · simp
+      -- Some facts about push
+      sorry
+    · simp
+    · simp [Proc.push, ← hcomp, compileFn, aps_push_commutes_tail, aps_push_commutes_append]
+    · simp [AtomicProcs.HasEmptyInputs]
+    · simp [Seq.Config.init]
+    · intros expr hexpr
+      simp [Seq.Config.init] at hexpr
+      simp only [← hexpr]
+      and_intros
+      · exact f.WellFormedBody
+      · simp only [compileFn.bodyComp, Seq.Config.init, ExprState.init]
+        apply aps_push_preserves_shape
+      · intros ap hap inp hinp
+        constructor
+        · intros val hval
+          have ⟨var, hvar_lookup, hvar_name⟩ := hval
+          simp [Seq.Config.init, ExprState.init] at hvar_lookup
+          sorry
+        · sorry
+      · exists [], AtomicProcs.pushAll Op _ _ initUpdates (compileFn.resultSteers Op χ V m n)
+        simp [joinM]
+        and_intros
+        · -- TODO: reason about steer pushes
+          sorry
+        · -- TODO: reason about HasDiffPathSuffix
+          sorry
+        · constructor
+
+theorem sim_step
+  (ec ec' : Seq.Config Op χ V S m n)
+  (pc : Dataflow.Config Op (ChanName χ) V S m n)
+  (hsim : SimR _ _ _ _ ec pc)
+  (hstep : Config.Step Op χ V S ec ec') :
+  ∃ pc',
+    Config.StepPlus Op (ChanName χ) V S pc pc' ∧
+    SimR _ _ _ _ ec' pc' := by
+  have ⟨
+    heq_state,
+    hmatch_fn,
+    ⟨
+      rest,
+      carryInLoop,
+      carryDecider,
+      carryInputs₁,
+      carryInputs₂,
+      carryOutputs,
+      ctxLeft,
+      ctxCurrent,
+      ctxRight,
+      hatoms,
+      hdag,
+      hcarry_false,
+      hcarry_true,
+      hrest,
+      hempty_ctxLeft,
+      hret,
+      hcont,
+    ⟩,
+  ⟩ := hsim
+  cases hexpr : ec.expr with
+  | ret vals =>
+    cases hstep
+    simp at hexpr
+  | cont expr =>
+    -- simp only [Expr.Step, hexpr] at hstep
+    have ⟨
+      hwf_expr,
+      hmatch_ctxCurrent,
+      hlive_vars,
+      hctxRight,
+    ⟩ := hcont expr hexpr
+    cases expr with
+    | ret vars => sorry
+    | tail => sorry
+    | op o args bind cont =>
+      -- simp only [Expr.Step, hexpr, Expr.step] at hstep
+      -- simp [Expr.compile] at hmatch_ctxCurrent
+      -- -- generalize hap :
+      -- --   AtomicProc.op o
+      -- --     (Vector.map (Expr.compile.liveVar χ V ec.estate.definedVars ec.estate.pathConds) args)
+      -- --     (Expr.compile.newVars χ ec.estate.definedVars ec.estate.pathConds bind).snd
+      -- --   = ap
+      -- -- simp only [hap] at hmatch_ctxCurrent
+      -- have ⟨ap, hap_mem, hap_match⟩ := aps_match_implies_exists_ap_match
+      --   _ _ _ _ _ _
+      --   (aps_match_symmetric _ _ _ hmatch_ctxCurrent)
+      --   List.mem_cons_self
+      -- simp [AtomicProc.MatchModBuffers] at hap_match
+      -- cases ap <;> simp at hap_match
+      -- rename_i o' inputs outputs
+      -- have ⟨heq_o, hap_match_inputs, hap_match_outputs⟩ := hap_match
+      -- have hmem_ap : AtomicProc.op o' inputs outputs ∈ pc.proc.atoms := by
+      --   simp only [hrest] at hatoms
+      --   simp [hatoms]
+      --   right; left
+      --   assumption
+      -- TODO: from hlive_vars
+      -- have hinputs : ∀ input ∈ inputs, ∃ var val,
+      --   some val = ec.estate.vars var ∧
+      --   input = (.var var (ec.estate.definedVars.count var) ec.estate.pathConds, [val]) := sorry
+      -- TODO: from `hinputs'` and `hmem_ap'`,
+      --       show that we can run the atomic process
+      --       and substitute the result to the remainder of `ctxCurrent`.
+      --       - `ctxLeft` remain unchanged due to DAG structure
+      --       - `ctxRight` remain unchanged due to ??? (different pathConds)
+      -- TODO: show that the result preserves the relational invariant...
+      sorry
+    | br => sorry
+
+theorem compile_refines
+  (f : Fn Op χ m n)
+  (p : Proc Op (ChanName χ) V m n)
+  (hcomp : compileFn Op χ V S f = p)
+  (s : S)
+  (args : Vector V m) :
+  Refines
+    (Config.init _ _ _ _ f s args)
+    (Config.init _ _ _ _ p s args)
+    (SimR _ _ _ _)
+    (Config.Step Op χ V S)
+    (Config.StepPlus Op (ChanName χ) V S) := by
+  constructor
+  · apply sim_init_config
+    exact hcomp
+  · intros ec pc ec' hstep
+    apply sim_step _ _ _ _ ec ec'
+    exact hstep
+
+end Wavelet.Simulation
